src/lowparse/LowParseExample6.Aux.fst
@@ -10,13 +10,32 @@ module L = FStar.List.Tot
 type cases : eqtype =
   | Case_A
   | Case_B
+  | Case_V2
+  | Case_V3
+  | Case_V4
+  | Case_V5
+  | Case_V6
+  | Case_V7
+  | Case_V8
+  | Case_V9
 
 inline_for_extraction
-let case_enum : LP.enum cases U8.t =
+let u8 : eqtype = U8.t
+
+inline_for_extraction
+let case_enum : LP.enum cases u8 =
   [@inline_let]
   let e : list (cases * U8.t) = [
     Case_A, 18uy;
     Case_B, 42uy;
+    Case_V2, 71uy;
+    Case_V3, 72uy;
+    Case_V4, 73uy;
+    Case_V5, 74uy;
+    Case_V6, 75uy;
+    Case_V7, 76uy;
+    Case_V8, 77uy;
+    Case_V9, 78uy;
   ]
   in
   [@inline_let]
@@ -34,14 +53,39 @@ type t =
   | A of (U8.t * U8.t)
   | B of case_B
   | C : LP.unknown_enum_repr case_enum -> U16.t -> t
+  | V2 of U16.t
+  | V3 of U16.t
+  | V4 of  U16.t
+  | V5 of U16.t
+  | V6 of U16.t
+  | V7 of U16.t
+  | V8 of U16.t
+  | V9 of U16.t
+
+inline_for_extraction
+unfold
+let known_case_as_case_enum
+  (x: cases { norm [delta; zeta; iota; primops] (LP.list_mem x (LP.list_map fst case_enum)) == true } )
+: Tot (LP.enum_key case_enum)
+= [@inline_let]
+  let _ = norm_spec [delta; zeta; iota; primops] (LP.list_mem x (LP.list_map fst case_enum)) in
+  x
 
 inline_for_extraction
 let cases_of_t
   (x: t)
 : Tot (LP.maybe_enum_key case_enum)
 = match x with
-  | A _ -> LP.Known Case_A
-  | B _ -> LP.Known Case_B
+  | A _ -> LP.Known (known_case_as_case_enum Case_A)
+  | B _ -> LP.Known (known_case_as_case_enum Case_B)
+  | V2 _ -> LP.Known (known_case_as_case_enum Case_V2)
+  | V3 _ -> LP.Known (known_case_as_case_enum Case_V3)
+  | V4 _ -> LP.Known (known_case_as_case_enum Case_V4)
+  | V5 _ -> LP.Known (known_case_as_case_enum Case_V5)
+  | V6 _ -> LP.Known (known_case_as_case_enum Case_V6)
+  | V7 _ -> LP.Known (known_case_as_case_enum Case_V7)
+  | V8 _ -> LP.Known (known_case_as_case_enum Case_V8)
+  | V9 _ -> LP.Known (known_case_as_case_enum Case_V9)
   | C x _ -> LP.Unknown x
 
 inline_for_extraction
@@ -51,6 +95,59 @@ let type_of_known_case
 = match x with
   | Case_A -> U8.t * U8.t
   | Case_B -> case_B
+  | Case_V2 -> U16.t
+  | Case_V3 -> U16.t
+  | Case_V4 -> U16.t
+  | Case_V5 -> U16.t
+  | Case_V6 -> U16.t
+  | Case_V7 -> U16.t
+  | Case_V8 -> U16.t
+  | Case_V9 -> U16.t
+
+unfold
+inline_for_extraction
+let to_type_of_known_case
+  (k: LP.enum_key case_enum)
+  (x: cases)
+  (q: squash ((k <: cases) == x))
+  (#x' : LP.maybe_enum_key case_enum)
+  (y: LP.dsum_type_of_tag' case_enum type_of_known_case U16.t x')
+: Pure (norm [delta_only [(`%type_of_known_case)]; iota] (type_of_known_case x))
+  (requires (LP.Known k == x'))
+  (ensures (fun y' -> y' == y))
+= [@inline_let]
+  let _ = norm_spec [delta_only [(`%type_of_known_case)] ; iota] (type_of_known_case k) in
+  y
+
+unfold
+inline_for_extraction
+let to_refine_with_tag (k: LP.maybe_enum_key case_enum) (x: t) : Pure (LP.refine_with_tag cases_of_t k)
+  (requires (
+    norm [delta; iota; zeta] (cases_of_t x) == k
+  ))
+  (ensures (fun y -> y == x))
+= [@inline_let]
+  let _ = norm_spec [delta; iota; zeta] (cases_of_t x) in
+  x
+
+inline_for_extraction
+let synth_known_case
+  (k: LP.enum_key case_enum)
+  (y: LP.dsum_type_of_tag' case_enum type_of_known_case U16.t (LP.Known k))
+: Tot (LP.refine_with_tag cases_of_t (LP.Known k))
+= [@inline_let]
+  let x = LP.Known k in
+  match k with
+  | Case_A -> to_refine_with_tag x (A (to_type_of_known_case k Case_A () y))
+  | Case_B -> to_refine_with_tag x (B (to_type_of_known_case k Case_B () y))
+  | Case_V2 -> to_refine_with_tag x (V2 (to_type_of_known_case k Case_V2 () y))
+  | Case_V3 -> to_refine_with_tag x (V3 (to_type_of_known_case k Case_V3 () y))
+  | Case_V4 -> to_refine_with_tag x (V4 (to_type_of_known_case k Case_V4 () y))
+  | Case_V5 -> to_refine_with_tag x (V5 (to_type_of_known_case k Case_V5 () y))
+  | Case_V6 -> to_refine_with_tag x (V6 (to_type_of_known_case k Case_V6 () y))
+  | Case_V7 -> to_refine_with_tag x (V7 (to_type_of_known_case k Case_V7 () y))
+  | Case_V8 -> to_refine_with_tag x (V8 (to_type_of_known_case k Case_V8 () y))
+  | Case_V9 -> to_refine_with_tag x (V9 (to_type_of_known_case k Case_V9 () y))
 
 inline_for_extraction
 let synth_case
@@ -58,9 +155,55 @@ let synth_case
   (y: LP.dsum_type_of_tag' case_enum type_of_known_case U16.t x)
 : Tot (LP.refine_with_tag cases_of_t x)
 = match x with
-  | LP.Known Case_A -> (A y <: t)
-  | LP.Known Case_B -> (B y <: t)
-  | LP.Unknown x -> (C x y <: t)
+  | LP.Known k -> synth_known_case k y
+  | LP.Unknown k -> to_refine_with_tag x (C k y)
+
+unfold
+inline_for_extraction
+let from_type_of_known_case
+  (x' : LP.enum_key case_enum)
+  (x: cases)
+  (y: norm [delta_only [(`%type_of_known_case)]; iota] (type_of_known_case x))
+: Pure (type_of_known_case x')
+  (requires (x == x'))
+  (ensures (fun y' -> y' == y))
+= [@inline_let]
+  let _ = norm_spec [delta_only [(`%type_of_known_case)] ; iota] (type_of_known_case x) in
+  y
+
+let synth_case_recip_pre
+  (k: LP.maybe_enum_key case_enum)
+  (x: LP.refine_with_tag cases_of_t k)
+: GTot bool
+= match k with
+  | LP.Known Case_A -> (A? x)
+  | LP.Known Case_B -> (B? x)
+  | LP.Known Case_V2 -> (V2? x)
+  | LP.Known Case_V3 -> (V3? x)
+  | LP.Known Case_V4 -> (V4? x)
+  | LP.Known Case_V5 -> (V5? x)
+  | LP.Known Case_V6 -> (V6? x)
+  | LP.Known Case_V7 -> (V7? x)
+  | LP.Known Case_V8 -> (V8? x)
+  | LP.Known Case_V9 -> (V9? x)
+  | _ -> (C? x)
+
+let synth_case_recip_pre_intro1
+  (k: LP.maybe_enum_key case_enum)
+: Tot (
+  (x: t) ->
+  Tot (squash (k == cases_of_t x ==> synth_case_recip_pre k x == true)))
+= _ by (LP.synth_case_recip_pre_tac ()) // note: the same tactic works for both closed and open sums
+
+let synth_case_recip_pre_intro
+  (k: LP.maybe_enum_key case_enum)
+  (x: LP.refine_with_tag cases_of_t k)
+: Lemma (synth_case_recip_pre k x == true)
+= norm_spec [delta; iota] (synth_case_recip_pre k x);
+  assert (k == cases_of_t x);
+  let _ = synth_case_recip_pre_intro1 k x in
+  assert (k == cases_of_t x ==> synth_case_recip_pre k x == true); // FIXME: this is a BUG in F*, this assert should not be needed
+  ()
 
 inline_for_extraction
 let synth_case_recip
@@ -68,15 +211,59 @@ let synth_case_recip
   (x: LP.refine_with_tag cases_of_t k)
 : Tot (LP.dsum_type_of_tag' case_enum type_of_known_case U16.t k)
 = match k with
-  | LP.Known Case_A ->
-    (match x with A y -> (y <: LP.dsum_type_of_tag' case_enum type_of_known_case U16.t k))
-  | LP.Known Case_B -> (match x with B y -> (y <: LP.dsum_type_of_tag' case_enum type_of_known_case U16.t k))
-  | LP.Unknown _ -> (match x with C _ y ->  (y <: LP.dsum_type_of_tag' case_enum type_of_known_case U16.t k))
+  | LP.Known k' ->
+    begin match k' with
+    | Case_A ->
+      [@inline_let]
+      let _ = synth_case_recip_pre_intro (LP.Known Case_A) x in
+      (match x with A y -> from_type_of_known_case k' Case_A y)
+    | Case_B ->
+      [@inline_let]
+      let _ = synth_case_recip_pre_intro (LP.Known Case_B) x in
+      (match x with B y -> from_type_of_known_case k' Case_B y)
+    | Case_V2 ->
+      [@inline_let]
+      let _ = synth_case_recip_pre_intro (LP.Known Case_V2) x in
+      (match x with V2 y -> from_type_of_known_case k' Case_V2 y)
+    | Case_V3 ->
+      [@inline_let]
+      let _ = synth_case_recip_pre_intro (LP.Known Case_V3) x in
+      (match x with V3 y -> from_type_of_known_case k' Case_V3 y)
+    | Case_V4 ->
+      [@inline_let]
+      let _ = synth_case_recip_pre_intro (LP.Known Case_V4) x in
+      (match x with V4 y -> from_type_of_known_case k' Case_V4 y)
+    | Case_V5 ->
+      [@inline_let]
+      let _ = synth_case_recip_pre_intro (LP.Known Case_V5) x in
+      (match x with V5 y -> from_type_of_known_case k' Case_V5 y)
+    | Case_V6 ->
+      [@inline_let]
+      let _ = synth_case_recip_pre_intro (LP.Known Case_V6) x in
+      (match x with V6 y -> from_type_of_known_case k' Case_V6 y)
+    | Case_V7 ->
+      [@inline_let]
+      let _ = synth_case_recip_pre_intro (LP.Known Case_V7) x in
+      (match x with V7 y -> from_type_of_known_case k' Case_V7 y)
+    | Case_V8 ->
+      [@inline_let]
+      let _ = synth_case_recip_pre_intro (LP.Known Case_V8) x in
+      (match x with V8 y -> from_type_of_known_case k' Case_V8 y)
+    | Case_V9 ->
+      [@inline_let]
+      let _ = synth_case_recip_pre_intro (LP.Known Case_V9) x in
+      (match x with V9 y -> from_type_of_known_case k' Case_V9 y)
+    end
+  | LP.Unknown z ->
+    [@inline_let]
+    let _ = synth_case_recip_pre_intro (LP.Unknown z) x in
+    (match x with C _ y ->  (y <: LP.dsum_type_of_tag' case_enum type_of_known_case U16.t k))
 
 inline_for_extraction
 let t_sum : LP.dsum
-= LP.make_dsum case_enum cases_of_t type_of_known_case U16.t synth_case synth_case_recip
-    (fun x y -> ())
+= LP.make_dsum' case_enum cases_of_t type_of_known_case U16.t synth_case synth_case_recip
+    (_ by (LP.make_dsum_synth_case_recip_synth_case_known_tac ()))
+    (_ by (LP.make_dsum_synth_case_recip_synth_case_unknown_tac ()))
     (fun x -> ())
 
 let parse_case_B_filter
@@ -93,6 +280,7 @@ let parse_known_cases
 = match x with
   | Case_A -> (| _, LP.parse_u8 `LP.nondep_then` LP.parse_u8 |)
   | Case_B -> (| _, parse_case_B |)
+  | _ -> (| _, LP.parse_u16 |)
 
 let parse_t : LP.parser _ t =
   LP.parse_dsum t_sum LP.parse_u8 parse_known_cases LP.parse_u16
@@ -109,6 +297,7 @@ let parse32_known_cases
 = match x with
   | Case_A -> LP.parse32_u8 `LP.parse32_nondep_then` LP.parse32_u8
   | Case_B -> parse32_cases_B
+  | _ -> LP.parse32_u16
 
 let parse32_t
 : LP.parser32 parse_t
@@ -123,6 +312,7 @@ let serialize_known_cases
 = match x with
   | Case_A -> LP.serialize_nondep_then _ LP.serialize_u8 () _ LP.serialize_u8
   | Case_B -> serialize_case_B
+  | _ -> LP.serialize_u16
 
 let serialize_t
 : LP.serializer parse_t
@@ -139,6 +329,7 @@ let serialize32_known_cases
 = match x with
   | Case_A -> LP.serialize32_nondep_then LP.serialize32_u8 () LP.serialize32_u8 ()
   | Case_B -> serialize32_case_B
+  | _ -> LP.serialize32_u16
 
 inline_for_extraction
 let serialize32_key: LP.serializer32 (LP.serialize_maybe_enum_key _ LP.serialize_u8 case_enum) =
@@ -146,7 +337,8 @@ let serialize32_key: LP.serializer32 (LP.serialize_maybe_enum_key _ LP.serialize
 
 let serialize32_t
 : LP.serializer32 serialize_t
-= assert_norm (LP.serializer32_sum_gen_precond (LP.get_parser_kind LP.parse_u8) (LP.weaken_parse_dsum_cases_kind t_sum parse_known_cases (LP.get_parser_kind LP.parse_u16)));
+= [@inline_let]
+  let _ = assert_norm (LP.serializer32_sum_gen_precond (LP.get_parser_kind LP.parse_u8) (LP.weaken_parse_dsum_cases_kind t_sum parse_known_cases (LP.get_parser_kind LP.parse_u16))) in
   LP.serialize32_dsum t_sum _ serialize32_key _ _ serialize32_known_cases LP.serialize32_u16 (_ by (LP.dep_enum_destr_tac ())) ()
 
 inline_for_extraction
@@ -160,6 +352,7 @@ let size32_known_cases
 = match x with
   | Case_A -> LP.size32_nondep_then LP.size32_u8 () LP.size32_u8
   | Case_B -> size32_case_B
+  | _ -> LP.size32_u16
 
 inline_for_extraction
 let size32_key : LP.size32 (LP.serialize_maybe_enum_key _ LP.serialize_u8 case_enum) =
@@ -167,7 +360,8 @@ let size32_key : LP.size32 (LP.serialize_maybe_enum_key _ LP.serialize_u8 case_e
 
 let size32_t
 : LP.size32 serialize_t
-= assert_norm (LP.size32_sum_gen_precond (LP.get_parser_kind LP.parse_u8) (LP.weaken_parse_dsum_cases_kind t_sum parse_known_cases (LP.get_parser_kind LP.parse_u16)));
+= [@inline_let]
+  let _ = assert_norm (LP.size32_sum_gen_precond (LP.get_parser_kind LP.parse_u8) (LP.weaken_parse_dsum_cases_kind t_sum parse_known_cases (LP.get_parser_kind LP.parse_u16))) in
   LP.size32_dsum t_sum _ size32_key _ _ size32_known_cases LP.size32_u16 (_ by (LP.dep_enum_destr_tac ())) ()
 
 (*
